Generalized grover, testing arithmetic circuits

SQIR/Testing.v
@@ -1,4 +1,4 @@
-Require Import Arith Vector Bvector Equality MSets OrderedTypeEx Lia.
+Require Import Arith NArith Vector Bvector Equality MSets OrderedTypeEx Lia.
 From QuickChick Require Import QuickChick.
 Require Import VSQIR Utilities.
 Import Vector (hd, tl).
@@ -12,6 +12,8 @@ Import VarSet.
 
 Open Scope vector_scope.
 Open Scope string_scope.
+Open Scope positive_scope.
+Open Scope N_scope.
 Open Scope nat_scope.
 Open Scope bool_scope.
 Open Scope exp_scope.
@@ -65,36 +67,92 @@ Fixpoint gen_bvector' {n} : G (Bvector n) :=
 Instance gen_bvector n : Gen (Bvector n) := {| arbitrary := gen_bvector' |}.
 
 (* The natural number represented in binary in the sequence of bits *)
-Fixpoint bvector2nat {n} : Bvector n -> nat :=
+Fixpoint bvector2n {n} : Bvector n -> N :=
   match n with
-  | 0 => fun _ => 0
-  | S n' => fun v => Nat.b2n (hd v) + 2 * bvector2nat (tl v)
+  | 0 => fun _ => N0
+  | S n' =>
+      fun v =>
+      let tl_n := bvector2n (tl v) in
+      if hd v
+      then N.succ_double tl_n
+      else N.double tl_n
   end.
 
 (* Represents the natural number in binary, trucating if necessary *)
-Fixpoint nat2bvector n : nat -> Bvector n :=
+Fixpoint n2bvector n : N -> Bvector n :=
   match n with
   | 0 => fun _ => Bnil
-  | S n' => fun i => Nat.odd i :: nat2bvector n' (i / 2)
+  | S n' => fun i => N.odd i :: n2bvector n' (N.div2 i)
   end.
 
-Lemma bvector2nat2bvector :
-  forall n v, nat2bvector n (bvector2nat v) = v.
+Lemma bvector2n2bvector :
+  forall n v, n2bvector n (bvector2n v) = v.
 Proof.
-  intros n. induction n; intros v; dependent destruction v; try reflexivity.
-  cbn - [ "*" Nat.div ].
+  intros n.
+  induction n as [| n IH]; intros v; dependent destruction v; try reflexivity.
+  cbn - [ N.mul N.div ].
   assert
     (forall h h' (t t' : Bvector n), h = h' -> t = t' -> h :: t = h' :: t').
   { intros. subst. reflexivity. }
-  apply H.
-  - destruct h; cbn - [ "*" ].
-    + rewrite Nat.odd_succ, Nat.even_spec. econstructor. reflexivity.
-    + rewrite <- Nat.negb_even, negb_false_iff, Nat.even_spec.
-      econstructor. reflexivity.
-  - rewrite Nat.add_b2n_double_div2. apply IHn.
+  apply H; destruct h; auto using Ndouble_plus_one_bit0, Ndouble_bit0.
+  - rewrite N.div2_succ_double. apply IH.
+  - rewrite N.div2_double. apply IH.
 Qed.
 
-(* Rotation of 0, multiplication by 1 *)
+Definition bvector2nat {n} (v : Bvector n) := N.to_nat (bvector2n v).
+
+(*
+Definition num_bits n :=
+  match n with
+  | N0 => 1
+  | Npos p => Pos.size_nat p
+  end.
+
+Lemma num_bits_le :
+  forall n p, num_bits n <= p <-> N.to_nat n < 2 ^ p.
+Proof.
+Abort. (* TODO *)
+*)
+
+Lemma double_size :
+  forall n, N.size_nat (N.double n) <= S (N.size_nat n).
+Proof.
+  intros [].
+  - simpl. lia.
+  - reflexivity.
+Qed.
+
+Lemma succ_double_size :
+  forall n, N.size_nat (N.succ_double n) = S (N.size_nat n).
+Proof. intros []; reflexivity. Qed.
+
+Lemma size_bvector2n :
+  forall n (v : Bvector n), N.size_nat (bvector2n v) <= n.
+Proof.
+  intros n. induction n as [| n IH]; intros v; simpl. try constructor.
+  dependent destruction v. simpl. destruct h.
+  - rewrite succ_double_size. auto using le_n_S.
+  - eauto using le_trans, double_size, le_n_S.
+Qed.
+
+(*
+Lemma size_div2_le :
+  forall i n, N.size_nat i <= S n <-> N.size_nat (N.div2 i) <= n.
+Proof.
+  intros i n.
+  split; intros H; generalize dependent i;
+  induction n as [| n IH]; intros [|[]] H; simpl in *; lia.
+Qed.
+ *)
+
+Lemma n2bvector2n :
+  forall n i, N.size_nat i <= n -> bvector2n (n2bvector n i) = i.
+Proof.
+  intros n. induction n as [| n IH]; try (intros [|[]]; simpl; lia).
+  intros [|[]] H; simpl; rewrite IH; simpl in *; try lia.
+Qed.
+
+(* Rotation of 0, scalar multiplication by 1 *)
 Definition zero_angle : rz_val :=
   fun _ => false.
 
@@ -114,15 +172,19 @@ Notation "x |-> vx , st" :=
     (eupdate st x vx) (at level 100, vx at next level, right associativity).
 Infix "|->" := (eupdate zero_state) (at level 100).
 
-(* Updates a whole variable rather than a single position *)
-Reserved Notation "x |=> vx , st" 
-    (at level 100, vx at next level, right associativity).
-Fixpoint update_var {n} (st : state) x : Bvector n -> state :=
+Definition next_pos : posi -> posi := fun '(x, i) => (x, S i).
+
+Fixpoint update_var' {n} (st : state) (x : posi) : Bvector n -> state :=
   match n with
   | 0 => fun _ => st
-  | S n' => fun vx => (x |=> tl vx, (x, n') |-> basis_val (hd vx), st)
-  end
-where "x |=> vx , st" := (update_var st x vx).
+  | S n' =>
+      fun vx => (x |-> basis_val (hd vx), update_var' st (next_pos x) (tl vx))
+  end.
+
+Definition update_var {n} st x : Bvector n -> state := update_var' st (x, 0).
+
+Notation "x |=> vx , st" :=
+    (update_var st x vx) (at level 100, vx at next level, right associativity).
 
 Infix "|=>" := (update_var zero_state) (at level 100).
 
@@ -254,7 +316,7 @@ Fixpoint get_exp_vars e :=
   end.
 
 (* Get the variables in a pexp *)
-Fixpoint get_vars e :=
+Fixpoint get_vars e : var_set :=
   match e with
   | Exp e' => get_exp_vars e'
   | QFT x => singleton x
@@ -292,6 +354,81 @@ Fixpoint get_prec (env : f_env) e :=
   | e1;; e2 => max (get_prec env e1) (get_prec env e2)
   end.
 
+Definition ospec m n := Bvector m -> Bvector n -> Prop.
+
+Definition fun_adheres {m n} f (s : ospec m n) :=
+  forall vx, s vx (f vx).
+
+Definition ospec_fun {m n} f : ospec m n :=
+  fun vx vy => f vx = vy.
+
+Lemma ospec_fun_adheres :
+  forall m n (f : Bvector m -> Bvector n), fun_adheres f (ospec_fun f).
+Proof. congruence. Qed.
+
+Definition ospec_bool {n} (s : Bvector n -> bool -> Prop) : ospec n 1 :=
+  fun vx vy => s vx (hd vy).
+
+Definition bool_fun_adheres {n} f (s : ospec n 1) :=
+  forall vx, s vx (f vx :: Bnil).
+
+Definition ospec_bool_fun {n} f : ospec n 1 :=
+  ospec_bool (fun vx b => f vx = b).
+
+Lemma ospec_bool_fun_adheres :
+  forall n (f : Bvector n -> bool), bool_fun_adheres f (ospec_bool_fun f).
+Proof.
+  intros n f vx. unfold ospec_bool_fun, ospec_bool. reflexivity.
+Qed.
+
+Definition ospec_n m n (s : N -> N -> Prop) : ospec m n :=
+  fun vx vy => s (bvector2n vx) (bvector2n vy).
+
+Definition n_fun_adheres {m n} f (s : ospec m n) :=
+  forall vx,
+  let ny := f (bvector2n vx) in N.size_nat ny <= n /\ s vx (n2bvector n ny).
+
+Definition ospec_n_fun m n f : ospec m n :=
+  ospec_n m n (fun nx ny => f nx = ny).
+
+Lemma ospec_n_fun_adheres :
+  forall m n (f : N -> N),
+  (forall nx, N.size_nat nx <= m -> N.size_nat (f nx) <= n) ->
+  n_fun_adheres f (ospec_n_fun m n f).
+Proof.
+  intros m n f H vx. simpl. split.
+  - auto using size_bvector2n.
+  - unfold ospec_n_fun, ospec_n. rewrite n2bvector2n; auto using size_bvector2n.
+Qed.
+
+Definition ospec_n_bool n (s : N -> bool -> Prop) : ospec n 1 :=
+  fun vx vy => s (bvector2n vx) (hd vy).
+
+Definition ospec_n_bool_fun n f : ospec n 1 :=
+  ospec_n_bool n (fun nx b => f nx = b).
+
+Definition is_oracle_fun x y env (f : Bvector (env x) -> Bvector (env y)) e :=
+  forall vx vy,
+  st_equiv (get_vars e) env (get_prec env e)
+      (prog_sem env e (x |=> vx, y |=> vy)) (x |=> vx, y |=> vy (+) f vx).
+
+Definition is_oracle x y env (s : ospec (env x) (env y)) e :=
+  exists f, fun_adheres f s /\ is_oracle_fun x y env f e.
+
+Definition is_oracle_bool x y env (s : ospec (env x) 1) e :=
+  exists H : env y = 1, is_oracle x y env (eq_rect_r (ospec (env x)) s H) e.
+
+(*
+Lemma is_oracle_fun_is_oracle :
+  forall x y env f e,
+  is_oracle_fun x y env f e <-> is_oracle x y env (ospec_fun f) e.
+Proof.
+  intros x y env f e. split.
+  - intros H. exists f. auto using ospec_fun_adheres.
+  - intros [f' [Ha Ho]].
+  H. exists f. auto using ospec_fun_adheres.
+Qed.
+
 (* Is the pexp an oracle for a function from Bvectors to Bvectors? *)
 Definition is_oracle x y env (f : Bvector (env x) -> Bvector (env y)) e :=
   forall vx vy,
@@ -303,8 +440,8 @@ Definition is_oracle_bool x y env (f : Bvector (env x) -> bool) e :=
   env y = 1 /\
   is_oracle x y env (fun v => Vector.const (f v) _) e.
 
-(* Is the pexp an oracle for a function from nats to nats? *)
-Definition is_oracle_nat x y env (f : nat -> nat) e :=
+(* Is the pexp an oracle for a function from N to N? *)
+Definition is_oracle_n x y env (f : N -> N) e :=
   is_oracle x y env (fun v => nat2bvector (env y) (f (bvector2nat v))) e.
 
 (* Is the pexp an oracle for a function from nats to bools? *)
@@ -317,6 +454,7 @@ Instance checkable_and {P Q : Prop} `{Checkable P} `{Checkable Q} :
   {|
     checker '(conj p q) := conjoin (checker p :: checker q :: nil)%list
   |}.
+ *)
 
 (* Example: an oracle for the "not" function *)
 Module NotExample.
@@ -327,6 +465,8 @@ Module NotExample.
   (* Given a bvector of length 1, negate its only element *)
   Example not_function (vx : Bvector 1) := negb (hd vx).
 
+  Example not_ospec := ospec_bool_fun not_function.
+
   (* An oracle for the "not" function *)
   Example not_oracle := Exp (X (x, 0); CNOT (x, 0) (y, 0); X (x, 0)).
 
@@ -335,7 +475,7 @@ Module NotExample.
     fun x' => if (x' =? x) || (x' =? y) then 1 else 0.
 
   Conjecture not_oracle_correct :
-    is_oracle_bool x y not_oracle_env not_function not_oracle.
+    is_oracle x y not_oracle_env not_ospec not_oracle.
 
 End NotExample.
 
@@ -343,3 +483,114 @@ End NotExample.
 (*
 QuickChick NotExample.not_oracle_correct.
 *)
+
+Infix "<*>" := kron (at level 40, only parsing).
+
+Definition nat_bool_to_n_bool f n : bool := f (N.to_nat n).
+
+Definition circuit_dim (env : f_env) e :=
+  list_sum (map env (elements (get_vars e))).
+
+Definition xy_first x y (env : f_env) (vs : vars) :=
+  let '(xstart, _, _, _) := vs x in
+  let '(ystart, _, _, _) := vs y in
+  xstart = 0 /\ ystart = env x.
+
+Lemma vkron_add :
+  forall n m f,
+  (forall i, i < n + m -> WF_Matrix (f i)) ->
+  vkron (n + m) f = vkron n f <*> vkron m (fun i => f (i + n)).
+Proof.
+  intros n m f H.
+  induction m as [| m IH]; simpl; Msimpl; auto with wf_db.
+  assert (forall i, i < n -> WF_Matrix (f i)) as Hn by (intros; apply H; lia).
+  assert (forall i, i < m -> WF_Matrix (f (i + n))) as Hm by (intros; apply H; lia).
+  assert (WF_Matrix (f (m + n))) as Hf by (intros; apply H; lia).
+  rewrite Nat.add_succ_r, <- kron_assoc; auto with wf_db. simpl.
+  rewrite IH by (intros; apply H; lia).
+  repeat apply f_equal. lia.
+Qed.
+
+Lemma update_var_eupdate_permute :
+  forall n x y i bx (vy : Bvector n) st,
+  x <> y -> ((x, i) |-> bx, y |=> vy, st) = (y |=> vy, (x, i) |-> bx, st).
+Proof.
+  intros n. unfold update_var. remember 0 as j. clear. generalize dependent j.
+  induction n as [| n IH]; try reflexivity.
+  intros j x y i bx vy st H. simpl.
+  rewrite eupdate_twice_neq by congruence.
+  rewrite IH by assumption. reflexivity.
+Qed.
+
+Lemma update_var_permute :
+  forall m n x y (vx : Bvector m) (vy : Bvector n) st,
+  x <> y -> (x |=> vx, y |=> vy, st) = (y |=> vy, x |=> vx, st).
+Proof.
+  intros m. unfold update_var. remember 0 as j.
+  intros n x y. replace (y, j) with (y, 0) by (subst; reflexivity).
+  generalize dependent y. generalize dependent x. generalize dependent n.
+  clear. generalize dependent j.
+  induction m as [| m IH]; try reflexivity.
+  intros j n x y vx vy st H. dependent destruction vx. simpl.
+  rewrite IH by assumption.
+Abort.
+
+Lemma trans_init_state :
+  forall m n dim x y avs rmax (vx : Bvector m) (vy : Bvector n),
+  x <> y ->
+  m + n <= dim ->
+  (forall i, i < m -> avs i = (x, i)) ->
+  (forall i, i < n -> avs (i + m) = (y, i)) ->
+  vkron dim (trans_state avs rmax (x |=> vx, y |=> vy)) =
+  @pad_vector (m + n)
+        dim
+        (basis_vector (2 ^ m) (bvector2nat vx) <*>
+           basis_vector (2 ^ n) (bvector2nat vy)).
+Proof.
+  intros m n dim x y avs rmax vx vy Nn He Hx Hy. unfold pad_vector.
+  remember (dim - (m + n)) as ancillae.
+  apply repad_lemma2 in Heqancillae; try assumption.
+  clear He. subst. rewrite vkron_add; auto using WF_trans_state.
+  rewrite Nat.pow_1_l. apply f_equal2.
+  - rewrite vkron_add; auto using WF_trans_state.
+    apply f_equal2.
+    + unfold trans_state. admit.
+Abort.
+(*
+    + rewrite update_var_permute by assumption. induction n as [| n IH].
+      * dependent destruction vy. simpl.
+        unfold bvector2nat. simpl. unfold basis_vector, I.
+        apply functional_extensionality.
+        intros []; apply functional_extensionality;
+        intros []; bdestruct_all; reflexivity.
+      * dependent destruction vy. unfold bvector2nat.
+        cbn - [ Nat.mul ].
+        rewrite vkron_eq with
+          (f' := fun i => trans_state avs rmax (y |=> vy, x |=> vx) (i + m)).
+        -- rewrite IH by (intros; apply Hy; lia).
+           destruct h.
+           ++ rewrite N2Nat.inj_succ_double.
+              replace (S (2 * _)) with (2 * N.to_nat (bvector2n vy) + 1) by lia.
+              rewrite <- (basis_vector_append_1 (2 ^ n)).
+              ** unfold bvector2nat. apply f_equal.
+                 unfold trans_state. rewrite Hy by constructor.
+                 rewrite eupdate_index_eq. simpl. Search turn_angle.
+*)
+
+Lemma todo :
+  forall x y env f e vs dim avs,
+  let '(p, _, _) := trans_pexp vs dim e avs in
+  S (env x) <= dim ->
+  xy_first x y env vs ->
+  is_oracle_bool x y env (ospec_n_bool_fun (env x) (nat_bool_to_n_bool f)) e ->
+  padded_boolean_oracle (env x) p f.
+Proof.
+  intros x y env f e vs dim avs.
+  destruct (trans_pexp vs dim e avs) as [[p vs'] avs'] eqn:E.
+  assert (p = fst (fst (trans_pexp vs dim e avs))) as Hp
+                                                   by (rewrite E; reflexivity).
+  intros Hd Hf [Hy H]. intros nx vy Hx. unfold pad_vector.
+  remember (dim - S (env x)) as ancillae.
+  apply repad_lemma2 in Heqancillae; try assumption.
+  rewrite Hp.
+Abort.
