SQIR/ArithTesting.v
@@ -1,0 +1,89 @@
+From Coq Require Import Arith NArith Vector Bvector.
+From QuickChick Require Import QuickChick.
+Require Import VSQIR Testing RZArith.
+
+Open Scope exp_scope.
+
+Fixpoint exp2 n :=
+  match n with
+  | 0 => 1%N
+  | S n' => N.double (exp2 n')
+  end.
+
+Lemma exp2_spec :
+  forall n, exp2 n = (2 ^ N.of_nat n)%N.
+Proof.
+  intros n. induction n as [| n IH].
+  - reflexivity.
+  - rewrite Nat2N.inj_succ, N.pow_succ_r'. cbn - [ N.mul ].
+    rewrite IH. apply N.double_spec.
+Qed.
+
+Definition add_bvector {n} (vn vn' : Bvector n) :=
+  n2bvector n ((bvector2n vn + bvector2n vn') mod (exp2 n))%N.
+
+Infix "[+]" := add_bvector (at level 50).
+
+Definition mul_bvector {n} (vn vn' : Bvector n) :=
+  n2bvector n ((bvector2n vn * bvector2n vn') mod (exp2 n))%N.
+
+Infix "[*]" := mul_bvector (at level 40).
+
+Module RzAdd.
+
+  Definition x := 0.
+  Definition y := 1.
+  Definition ex := 2.
+
+  Definition mod_add_circ n :=
+    Exp (Rev x; Rev y);;
+    QFT x;;
+    Exp (rz_full_adder x n y);;
+    RQFT x;;
+    Exp (Rev y; Rev x).
+
+  Definition mod_add_env n : f_env := fun _ => n.
+
+  Definition mod_add_prec n : nat := get_prec (mod_add_env n) (mod_add_circ n).
+
+  Conjecture mod_add_spec :
+    forall (n : nat) (vx vy : Bvector n),
+    st_equiv (get_vars (mod_add_circ n)) (mod_add_env n) (mod_add_prec n)
+      (prog_sem (fun _ => n) (mod_add_circ n) (x |=> vx, y |=> vy))
+          (x |=> vx [+] vy, y |=> vy).
+
+End RzAdd.
+
+(* QuickChick RzAdd.mod_add_spec. *)
+
+Module ModMul.
+
+  Definition mod_mul n n' d := (n * n' mod (2 ^ d))%N.
+
+  Definition mod_mul_vec {n} (vn vn' : Bvector n) :=
+    n2bvector n (mod_mul (bvector2n vn) (bvector2n vn') (N.of_nat n)).
+
+  Definition x := 0.
+  Definition y := 1.
+  Definition re := 2.
+  Definition ex := 3.
+
+  Definition mod_mul_circ n := nat_full_mult n x y re ex.
+
+  Definition mod_mul_vars n := get_vars (mod_mul_circ n).
+
+  Definition mod_mul_env n : f_env := fun _ => n.
+
+  Definition mod_mul_prec n : nat := get_prec (mod_mul_env n) (mod_mul_circ n).
+
+  Conjecture mod_mul_spec :
+    forall (n : nat) (vx vy vre : Bvector n),
+    st_equiv (mod_mul_vars n) (mod_mul_env n) (mod_mul_prec n)
+      (prog_sem (mod_mul_env n) (mod_mul_circ n)
+        (x |=> vx, y |=> vy, re |=> vre))
+      (x |=> vx, y |=> vy, re |=> vre [+] vx [*] vy).
+
+End ModMul.
+
+QuickChickWith (updMaxSuccess stdArgs 1) (ModMul.mod_mul_spec 16).
+
